@prefix : <http://www.w3.org/ns/td#> .
@prefix dc: <http://purl.org/dc/elements/1.1/> .
@prefix vs: <http://www.w3.org/2003/06/sw-vocab-status/ns#> .
@prefix owl: <http://www.w3.org/2002/07/owl#> .
@prefix rdf: <http://www.w3.org/1999/02/22-rdf-syntax-ns#> .
@prefix xml: <http://www.w3.org/XML/1998/namespace> .
@prefix xsd: <http://www.w3.org/2001/XMLSchema#> .
@prefix foaf: <http://xmlns.com/foaf/0.1/> .
@prefix prov: <http://www.w3.org/ns/prov#> .
@prefix rdfs: <http://www.w3.org/2000/01/rdf-schema#> .
@prefix vann: <http://purl.org/vocab/vann/> .
@prefix dcterms: <http://purl.org/dc/terms/> .

<http://www.w3.org/ns/td#> rdf:type owl:Ontology ;
                           
                           owl:versionInfo "0.0.1" ;
                           
                           vann:preferredNamespacePrefix "td" ;
                           
                           dc:title "Ontology model for Web of Things"@en ;
                           
                           rdfs:comment "This ontology aims to model the Web of Things domain according to the W3C Interest Group (http://w3c.github.io/wot/)"@en ;
                           
                           vann:preferredNamespaceUri "http://www.w3.org/ns/td#" ;
                           
                           dcterms:license <http://purl.org/NET/rdflicense/cc-by4.0> ;
                           
                           dcterms:creator <http://purl.org/net/mpoveda> ,
                                           <http://www.garcia-castro.com/foaf.rdf#me> ;
                           
                           dcterms:contributor <http://www.oeg-upm.net/index.php/en/universitystaff/402-fserena/> ;
                           
                           dc:publisher <https://www.w3.org/WoT/WG/> .


#################################################################
#
#    Annotation properties
#
#################################################################


###  http://www.w3.org/2003/06/sw-vocab-status/ns#term_status

vs:term_status rdf:type owl:AnnotationProperty .





#################################################################
#
#    Object Properties
#
#################################################################


###  http://www.w3.org/ns/td#actions

:actions rdf:type owl:ObjectProperty ;
         
         rdfs:label "actions" ;
         
         rdfs:comment "Keeps all Action-based interaction pattern of the Thing." ;
         
         rdfs:range :Action ;
         
         rdfs:domain :Thing ;
         
         rdfs:subPropertyOf :interactions .



###  http://www.w3.org/ns/td#events

:events rdf:type owl:ObjectProperty ;
        
        rdfs:label "events" ;
        
        rdfs:comment "Keeps all Event-based interaction pattern of the Thing." ;
        
        rdfs:subPropertyOf :interactions .



###  http://www.w3.org/ns/td#forms

:forms rdf:type owl:ObjectProperty ;
       
       rdfs:label "forms"@en ;
       
       rdfs:comment "Indicates one or more endpoints from which an interaction pattern is accessible"@en .



###  http://www.w3.org/ns/td#input

:input rdf:type owl:ObjectProperty ;
       
       rdfs:label "input"@en ;
       
       rdfs:comment "link to the n-ary class that allows the declaration of the accepted data type of an action."@en ;
       
       rdfs:range :Property ;
       
       rdfs:domain :Thing .



###  http://www.w3.org/ns/td#interactions

:interactions rdf:type owl:ObjectProperty .



###  http://www.w3.org/ns/td#items

:items rdf:type owl:ObjectProperty ;
       
       rdfs:label "items" ;
       
       rdfs:comment "Used to defines characteristics of an array." ;
       
       rdfs:range :Property ;
       
       rdfs:domain :Thing .



###  http://www.w3.org/ns/td#links

:links rdf:type owl:ObjectProperty ;
       
       rdfs:label "links" ;
       
       rdfs:comment "provides Web links to arbitrary resources that relate to the specified Thing Description." .



###  http://www.w3.org/ns/td#objectSchemaProperties

:objectSchemaProperties rdf:type owl:ObjectProperty ;
                        
                        rdfs:label "properties" ;
                        
                        rdfs:comment "Data schema nested definitions" .



###  http://www.w3.org/ns/td#output

:output rdf:type owl:ObjectProperty ;
        
        rdfs:label "output"@en ;
        
        rdfs:comment "link to the n-ary class that allows the declaration of the data type returned by an action."@en ;
        
        rdfs:range :Property ;
        
        rdfs:domain :Thing .



###  http://www.w3.org/ns/td#properties

:properties rdf:type owl:ObjectProperty ;
            
            rdfs:label "properties" ;
            
            rdfs:comment "Keeps all Property-based interaction pattern of the Thing." ;
            
            rdfs:range :Property ;
            
            rdfs:domain :Thing ;
            
            rdfs:subPropertyOf :interactions .



###  http://www.w3.org/ns/td#schema

:schema rdf:type owl:ObjectProperty ;
        
        rdfs:label "schema"@en ;
        
        rdfs:comment "schema definition for values of the given object schema property."@en ;
        
        rdfs:range :Property .



###  http://www.w3.org/ns/td#securityDefinition

:securityDefinition rdf:type owl:ObjectProperty ;
                    
                    rdfs:label "securityDefinitions"@en ;
                    
                    rdfs:comment "Links a given Thing to the security information that indicates the access metadata information for securely transmitting information via all the resources of the Thing."@en .





#################################################################
#
#    Data properties
#
#################################################################


###  http://www.w3.org/ns/td#anchor

:anchor rdf:type owl:DatatypeProperty ;
        
        rdfs:label "anchor" ;
        
        rdfs:comment "By default, the context of a link is the URL of the representation it is associated with, and is serialised as a URI. When present, the anchor parameter overrides this with another URI, such as a fragment of this resource, or a third resource (i.e., when the anchor value is an absolute URI)." .



###  http://www.w3.org/ns/td#base

:base rdf:type owl:DatatypeProperty ;
      
      rdfs:label "base"@en ;
      
      rdfs:comment "Define base URI that is valid for all defined local interaction resources. All other URIs in the TD must then be resolved using the algorithm defined in [[!RFC3986]]. This field is optional."@en ;
      
      rdfs:range xsd:anyURI .



###  http://www.w3.org/ns/td#const

:const rdf:type owl:DatatypeProperty ;
       
       rdfs:label "const" ;
       
       rdfs:comment "Provides a constant value." ;
       
       rdfs:range rdfs:Literal .



###  http://www.w3.org/ns/td#description

:description rdf:type owl:DatatypeProperty ;
             
             rdfs:label "description" ;
             
             rdfs:comment "Provides additionel (human) readable information." ;
             
             rdfs:range xsd:string .



###  http://www.w3.org/ns/td#enum

:enum rdf:type owl:DatatypeProperty ;
      
      rdfs:label "enum" ;
      
      rdfs:comment "Restricted set of values provided as array." ;
      
      rdfs:range rdfs:Literal .



###  http://www.w3.org/ns/td#href

:href rdf:type owl:DatatypeProperty ,
               owl:FunctionalProperty ;
      
      rdfs:label "href"@en ;
      
      rdfs:comment "URI of the endpoint where an interaction pattern is provided"@en ;
      
      rdfs:range xsd:anyURI .



###  http://www.w3.org/ns/td#id

:id rdf:type owl:DatatypeProperty ;
    
    rdfs:label "id" ;
    
    rdfs:comment "Defines unique URI (includes also URNs) ID of the Thing." ;
    
    rdfs:range xsd:anyURI .



###  http://www.w3.org/ns/td#in

:in rdf:type owl:DatatypeProperty ;
    
    rdfs:label "in" ;
    
    rdfs:comment "Specifies location of the authentication information" ;
    
    rdfs:range xsd:string .



###  http://www.w3.org/ns/td#label

:label rdf:type owl:DatatypeProperty ;
       
       rdfs:label "label" ;
       
       rdfs:comment "Provides a label (e.g., display a text for UI representation) of the interaction pattern." ;
       
       rdfs:range xsd:string .



###  http://www.w3.org/ns/td#maxItems

:maxItems rdf:type owl:DatatypeProperty ;
          
          rdfs:label "maxItems" ;
          
          rdfs:comment "Defines the maximum number of itmes that have to be in the array." ;
          
          rdfs:range xsd:unsignedInt .



###  http://www.w3.org/ns/td#maximum

:maximum rdf:type owl:DatatypeProperty ;
         
         rdfs:label "maximum" ;
         
         rdfs:comment "Specifies a maximum numeric value. Only applicable for associated number or integer types." ;
         
         rdfs:seeAlso <http://schema.org/maxValue> ;
         
         rdfs:range xsd:double .



###  http://www.w3.org/ns/td#mediaType

:mediaType rdf:type owl:DatatypeProperty ;
           
           rdfs:label "mediaType"@en ;
           
           rdfs:comment "Assign underlying media type of the interaction pattern based on IANA (https://www.iana.org/assignments/media-types/media-types.xhtml)"@en ;
           
           rdfs:range xsd:string .



###  http://www.w3.org/ns/td#minItems

:minItems rdf:type owl:DatatypeProperty ;
          
          rdfs:label "minItems" ;
          
          rdfs:comment "Defines the minimum number of itmes that have to be in the array." ;
          
          rdfs:range xsd:unsignedInt .



###  http://www.w3.org/ns/td#minimum

:minimum rdf:type owl:DatatypeProperty ;
         
         rdfs:label "minimum" ;
         
         rdfs:comment "Specifies a minimum numeric value. Only applicable for associated number or integer types." ;
         
         rdfs:seeAlso <http://schema.org/minValue> ;
         
         rdfs:range xsd:double .



###  http://www.w3.org/ns/td#name

:name rdf:type owl:DatatypeProperty ;
      
      rdfs:label "name"@en ;
      
      rdfs:comment "Name of the Thing or interaction pattern (must be a valid keyword to be used in the scripting API)" ;
      
      rdfs:range xsd:string .



###  http://www.w3.org/ns/td#observable

:observable rdf:type owl:DatatypeProperty ,
                     owl:FunctionalProperty ;
            
            rdfs:label "observable"@en ;
            
            rdfs:comment "Indicates whether a remote servient can subscribe to (\"observe\") the Property, to receive change notifications or periodic updates (true/false). "@en ;
            
            rdfs:range xsd:boolean .



###  http://www.w3.org/ns/td#rel

:rel rdf:type owl:DatatypeProperty ;
     
     rdfs:label "rel"@en ;
     
     rdfs:comment """Indicates the expected result of performing the operation described by the form.

For example, the Property interaction allows get and set operations. The protocol binding may contain a form for the get operation and a different form for the set operation. The value of the \"rel\" attribute of the form indicates which form is which and allows the client to select the correct form for the oeration required"""@en ;
     
     rdfs:range xsd:string .



###  http://www.w3.org/ns/td#required

:required rdf:type owl:DatatypeProperty ;
          
          rdfs:label "required" ;
          
          rdfs:comment "Defines which members of the object type are required/mandatory." ;
          
          rdfs:range xsd:string .



###  http://www.w3.org/ns/td#scheme

:scheme rdf:type owl:DatatypeProperty ;
        
        rdfs:label "scheme" ;
        
        rdfs:comment "Identification of security scheme (e.g., basic, digest, and oauth2)." .



###  http://www.w3.org/ns/td#security

:security rdf:type owl:DatatypeProperty ;
          
          rdfs:label "security" ;
          
          rdfs:comment "Defines the security requirements of the interacions by making a reference to the top level securityDefinition" ;
          
          rdfs:range rdfs:Literal .



###  http://www.w3.org/ns/td#support

:support rdf:type owl:DatatypeProperty ;
         
         rdfs:label "support" ;
         
         rdfs:comment "Provides information about TD maintainer (e.g., author, link or telephon number to get support, etc)." .



###  http://www.w3.org/ns/td#type

:type rdf:type owl:DatatypeProperty ;
      
      rdfs:label "type" ;
      
      rdfs:comment "Assignment of JSON-based data types that are compatible with JSON Schema (boolean, integer, number, string, object, array, null)." ;
      
      rdfs:range xsd:string .



###  http://www.w3.org/ns/td#writable

:writable rdf:type owl:DatatypeProperty ,
                   owl:FunctionalProperty ;
          
          rdfs:label "writable"@en ;
          
          rdfs:comment "Boolean value that indicates whether a property is writable (=true) or not (=false)"@en ;
          
          rdfs:range xsd:boolean .





#################################################################
#
#    Classes
#
#################################################################


###  http://www.w3.org/ns/td#Action

:Action rdf:type owl:Class ;
        
        rdfs:label "Action"@en ;
        
        rdfs:subClassOf :InteractionPattern ,
                        [ rdf:type owl:Restriction ;
                          owl:onProperty :output ;
                          owl:allValuesFrom :Property
                        ] ,
                        [ rdf:type owl:Restriction ;
                          owl:onProperty :input ;
                          owl:allValuesFrom :Property
                        ] ;
        
        rdfs:comment "Actions offer functions of the Thing. These functions may manipulate the interal state of a Thing in a way that is not possible through setting Properties. Examples are changing internal state that is not exposed as Property, changing multiple Properties, changing Properties over time or with a process that shall not be disclosed. Actions may also be pure functions, that is, they do not use any internal state at all, e.g., for processing input data and returning the result directly."@en .



###  http://www.w3.org/ns/td#ArraySchema

:ArraySchema rdf:type owl:Class ;
             
             rdfs:subClassOf :DataSchema ,
                             [ rdf:type owl:Restriction ;
                               owl:onProperty :maxItems ;
                               owl:allValuesFrom xsd:unsignedInt
                             ] ,
                             [ rdf:type owl:Restriction ;
                               owl:onProperty :minItems ;
                               owl:allValuesFrom xsd:unsignedInt
                             ] ,
                             [ rdf:type owl:Restriction ;
                               owl:onProperty :items ;
                               owl:allValuesFrom :DataSchema
                             ] ;
             
             rdfs:comment "A JSON array specification (\"type\": \"array\")." .



###  http://www.w3.org/ns/td#BooleanSchema

:BooleanSchema rdf:type owl:Class ;
               
               rdfs:subClassOf :DataSchema ;
               
               rdfs:comment "A JSON boolean value specification (\"type\": \"boolean\")." .



###  http://www.w3.org/ns/td#DataSchema

:DataSchema rdf:type owl:Class ;
            
            rdfs:subClassOf [ rdf:type owl:Restriction ;
                              owl:onProperty :const ;
                              owl:allValuesFrom rdfs:Literal
                            ] ,
                            [ rdf:type owl:Restriction ;
                              owl:onProperty :type ;
                              owl:allValuesFrom xsd:string
                            ] ,
                            [ rdf:type owl:Restriction ;
                              owl:onProperty :enum ;
                              owl:allValuesFrom rdfs:Literal
                            ] ;
            
            rdfs:comment "Any JSON value specification." .



###  http://www.w3.org/ns/td#Event

:Event rdf:type owl:Class ;
       
       rdfs:label "Event" ;
       
       rdfs:subClassOf :InteractionPattern ;
       
       rdfs:comment "The Event Interaction Pattern describes event sources that asynchronously push messages. Here not state, but state transitions (events) are communicated (e.g., \"clicked\"). Events may be triggered by internal state changes that are not exposed as Properties. Events usually follow strong consistency, where messages need to be queued to ensure eventual delivery of all occured events." .



###  http://www.w3.org/ns/td#Form

:Form rdf:type owl:Class ;
      
      rdfs:label "Form"@en ;
      
      rdfs:subClassOf [ rdf:type owl:Restriction ;
                        owl:onProperty :href ;
                        owl:allValuesFrom xsd:anyURI
                      ] ,
                      [ rdf:type owl:Restriction ;
                        owl:onProperty :security ;
                        owl:allValuesFrom xsd:string
                      ] ,
                      [ rdf:type owl:Restriction ;
                        owl:onProperty :mediaType ;
                        owl:allValuesFrom xsd:string
                      ] ,
                      [ rdf:type owl:Restriction ;
                        owl:onProperty :rel ;
                        owl:allValuesFrom xsd:string
                      ] ,
                      [ rdf:type owl:Restriction ;
                        owl:onProperty :href ;
                        owl:someValuesFrom xsd:anyURI
                      ] ;
      
      rdfs:comment "Communication metadata where a service can be accessed by a client application. An interaction might have more than one form."@en .



###  http://www.w3.org/ns/td#IntegerSchema

:IntegerSchema rdf:type owl:Class ;
               
               rdfs:subClassOf :DataSchema ,
                               :NumberSchema ,
                               [ rdf:type owl:Restriction ;
                                 owl:onProperty :minimum ;
                                 owl:allValuesFrom xsd:integer
                               ] ,
                               [ rdf:type owl:Restriction ;
                                 owl:onProperty :maximum ;
                                 owl:allValuesFrom xsd:integer
                               ] ;
               
               rdfs:comment "A JSON integer value specification, i.e. numbers without a fractional part (\"type\": \"integer\")." .



###  http://www.w3.org/ns/td#InteractionPattern

:InteractionPattern rdf:type owl:Class ;
                    
                    rdfs:label "InteractionPattern" ;
                    
                    rdfs:subClassOf [ rdf:type owl:Restriction ;
                                      owl:onProperty :forms ;
                                      owl:allValuesFrom :Form
                                    ] ,
                                    [ rdf:type owl:Restriction ;
                                      owl:onProperty :label ;
                                      owl:allValuesFrom xsd:string
                                    ] ,
                                    [ rdf:type owl:Restriction ;
                                      owl:onProperty :description ;
                                      owl:allValuesFrom xsd:string
                                    ] ;
                    
                    rdfs:comment "Three interaction patterns are defined as subclasses: Property, Action and Event. When a concrete Property, Action or Event is defined in a Thing Description, it is called an \\\"interaction resource\\\". Interactions between Things can be as simple as one Thing accessing another Thing's data to get or (in the case the data is also writable) change representation of data such as metadata, status or mode. A Thing may also be interested in getting asynchronously notified of future changes in another Thing, or may want to initiate a process served in another Thing that may take some time to complete and monitor the progress. Interactions between Things may involve exchanges of data between them. This data can be either given as input by the client Thing, returned as output by the server Thing or both."@en .



###  http://www.w3.org/ns/td#Link

:Link rdf:type owl:Class ;
      
      rdfs:label "Link" ;
      
      rdfs:subClassOf [ rdf:type owl:Restriction ;
                        owl:onProperty :mediaType ;
                        owl:allValuesFrom xsd:string
                      ] ,
                      [ rdf:type owl:Restriction ;
                        owl:onProperty :href ;
                        owl:allValuesFrom xsd:anyURI
                      ] ,
                      [ rdf:type owl:Restriction ;
                        owl:onProperty :anchor ;
                        owl:allValuesFrom xsd:anyURI
                      ] ,
                      [ rdf:type owl:Restriction ;
                        owl:onProperty :rel ;
                        owl:allValuesFrom xsd:string
                      ] ,
                      [ rdf:type owl:Restriction ;
                        owl:onProperty :href ;
                        owl:someValuesFrom xsd:anyURI
                      ] ;
      
      rdfs:comment "A Web link, as specified by IETF RFC 8288 (https://tools.ietf.org/html/rfc8288)." .



###  http://www.w3.org/ns/td#NumberSchema

:NumberSchema rdf:type owl:Class ;
              
              rdfs:subClassOf :DataSchema ,
                              [ rdf:type owl:Restriction ;
                                owl:onProperty :maximum ;
                                owl:allValuesFrom [ rdf:type rdfs:Datatype ;
                                                    owl:unionOf ( xsd:double
                                                                  xsd:integer
                                                                )
                                                  ]
                              ] ,
                              [ rdf:type owl:Restriction ;
                                owl:onProperty :minimum ;
                                owl:allValuesFrom [ rdf:type rdfs:Datatype ;
                                                    owl:unionOf ( xsd:double
                                                                  xsd:integer
                                                                )
                                                  ]
                              ] ;
              
              rdfs:comment "A JSON number value specification (\"type\": \"number\")." .



###  http://www.w3.org/ns/td#ObjectSchema

:ObjectSchema rdf:type owl:Class ;
              
              rdfs:subClassOf :DataSchema ,
                              [ rdf:type owl:Restriction ;
                                owl:onProperty :required ;
                                owl:allValuesFrom xsd:string
                              ] ,
                              [ rdf:type owl:Restriction ;
                                owl:onProperty :properties ;
                                owl:allValuesFrom :DataSchema
                              ] ;
              
              rdfs:comment "A JSON object specification (\"type\": \"object\")." .



###  http://www.w3.org/ns/td#Property

:Property rdf:type owl:Class ;
          
          rdfs:label "Property"@en ;
          
          rdfs:subClassOf :InteractionPattern ,
                          [ rdf:type owl:Restriction ;
                            owl:onProperty :writable ;
                            owl:allValuesFrom xsd:boolean
                          ] ,
                          [ rdf:type owl:Restriction ;
                            owl:onProperty :observable ;
                            owl:allValuesFrom xsd:boolean
                          ] ;
          
          rdfs:comment "Properties expose internal state of a Thing that can be directly accessed (get) and optionally manipulated (set). In addition, Things can also choose to make Properties observable by pushing the new state (not an event) after a change; this must follow eventual consistency (also see CAP Theorem)."@en .



###  http://www.w3.org/ns/td#Security

:Security rdf:type owl:Class ;
          
          rdfs:label "Security"@en ;
          
          rdfs:subClassOf [ rdf:type owl:Restriction ;
                            owl:onProperty :in ;
                            owl:allValuesFrom xsd:string
                          ] ,
                          [ rdf:type owl:Restriction ;
                            owl:onProperty :scheme ;
                            owl:allValuesFrom xsd:string
                          ] ;
          
          rdfs:comment "The (optional) security field can be used to provide access metadata (self-contained) information of the Thing for securely transmitting information via all its resources. Also see Section Security Consideration. Definition taken from http://w3c.github.io/wot/current-practices/wot-practices#security-metadata"@en ;
          
          vs:term_status "testing"@en .



###  http://www.w3.org/ns/td#SimpleDataSchema

:SimpleDataSchema rdf:type owl:Class ;
                  
                  owl:equivalentClass [ rdf:type owl:Class ;
                                        owl:unionOf ( :BooleanSchema
                                                      :NumberSchema
                                                      :StringSchema
                                                    )
                                      ] ;
                  
                  rdfs:subClassOf :DataSchema ;
                  
                  rdfs:seeAlso <http://schema.org/PropertyValueSpecification> .



###  http://www.w3.org/ns/td#StringSchema

:StringSchema rdf:type owl:Class ;
              
              rdfs:subClassOf :DataSchema ;
              
              rdfs:comment "A JSON string value specification (\"type\": \"string\")." .



###  http://www.w3.org/ns/td#Thing

:Thing rdf:type owl:Class ;
       
       rdfs:label "Thing"@en ;
       
       rdfs:subClassOf [ rdf:type owl:Restriction ;
                         owl:onProperty :id ;
                         owl:allValuesFrom xsd:string
                       ] ,
                       [ rdf:type owl:Restriction ;
                         owl:onProperty :name ;
                         owl:someValuesFrom xsd:string
                       ] ,
                       [ rdf:type owl:Restriction ;
                         owl:onProperty :properties ;
                         owl:allValuesFrom :Property
                       ] ,
                       [ rdf:type owl:Restriction ;
                         owl:onProperty :events ;
                         owl:allValuesFrom :Property
                       ] ,
                       [ rdf:type owl:Restriction ;
                         owl:onProperty :links ;
                         owl:allValuesFrom :Link
                       ] ,
                       [ rdf:type owl:Restriction ;
                         owl:onProperty :description ;
                         owl:allValuesFrom xsd:string
                       ] ,
                       [ rdf:type owl:Restriction ;
                         owl:onProperty :support ;
                         owl:allValuesFrom xsd:string
                       ] ,
                       [ rdf:type owl:Restriction ;
                         owl:onProperty :base ;
                         owl:allValuesFrom xsd:anyURI
                       ] ,
                       [ rdf:type owl:Restriction ;
                         owl:onProperty :securityDefinition ;
                         owl:allValuesFrom :Security
                       ] ,
                       [ rdf:type owl:Restriction ;
                         owl:onProperty :actions ;
                         owl:allValuesFrom :Action
                       ] ;
       
       rdfs:comment "Describes a physical and/or virtual Thing (may represent one or more physical and / or virtual Things) in the Web of Thing context."@en .




###  Generated by the OWL API (version 3.4.2) http://owlapi.sourceforge.net

