@prefix : <http://www.w3.org/ns/web-linking#> .
@prefix owl: <http://www.w3.org/2002/07/owl#> .
@prefix rdf: <http://www.w3.org/1999/02/22-rdf-syntax-ns#> .
@prefix xml: <http://www.w3.org/XML/1998/namespace> .
@prefix xsd: <http://www.w3.org/2001/XMLSchema#> .
@prefix rdfs: <http://www.w3.org/2000/01/rdf-schema#> .

<http://www.w3.org/ns/web-linking> rdf:type owl:Ontology ;
                                    rdfs:comment "Ontology designed to provide an RDF representation of Web links, in particular links expressed in the CoRE Link format." ;
                                    rdfs:label "Web Linking Ontology" .

#################################################################
#    Data properties
#################################################################

###  http://www.w3.org/ns/web-linking#anchor
:anchor rdf:type owl:DatatypeProperty ;
        rdfs:domain :Link ;
        rdfs:range xsd:anyURI ;
        rdfs:comment "By default, the context, or anchor, of a link conveyed in the Link header field is the URL of the representation it is associated with, as defined in RFC7231, Section 3.1.4.1, and is serialized as a URI." ;
        rdfs:label "anchor" .


###  http://www.w3.org/ns/web-linking#href
:href rdf:type owl:DatatypeProperty ;
      rdfs:domain :Link ;
      rdfs:range xsd:anyURI ;
      rdfs:comment "Each link-value conveys one target IRI as a URI-Reference (after conversion to one, if necessary; see RFC3987, Section 3.1) inside angle brackets (\"<>\")." ;
      rdfs:label "href" .


###  http://www.w3.org/ns/web-linking#rel
:rel rdf:type owl:DatatypeProperty ;
     rdfs:domain :Link ;
     rdfs:comment "A link relation type identifies the semantics of a link." ;
     rdfs:label "rel" .


###  http://www.w3.org/ns/web-linking#type
:type rdf:type owl:DatatypeProperty ;
      rdfs:domain :Link ;
      rdfs:range xsd:string ;
      rdfs:comment "Target attribute providing a hint indicating what the media type [IANA-MEDIA-TYPES] of the result of dereferencing the link should be." ;
      rdfs:label "type" .


#################################################################
#    Classes
#################################################################

###  http://www.w3.org/ns/web-linking#Link
:Link rdf:type owl:Class ;
      rdfs:comment "A link can be viewed as a statement of the form \"link context has a link relation type resource at link target, which has target attributes\"." ;
      rdfs:label "Link" .


###  Generated by the OWL API (version 4.5.9.2019-02-01T07:24:44Z) https://github.com/owlcs/owlapi
